src/Layers/CacheLayer/Definitions.v
@@ -3,41 +3,41 @@ Import ListNotations.
 
 Set Implicit Arguments.
   
-  Inductive token :=
-  | Crash : token
-  | Cont : token.
+  Inductive token' :=
+  | Crash : token'
+  | Cont : token'.
 
-  Definition token_dec : forall (t t': token), {t=t'}+{t<>t'}.
+  Definition token_dec' : forall (t t': token'), {t=t'}+{t<>t'}.
     decide equality.
   Defined.
 
-  Definition oracle := list token.  
+  Definition oracle' := list token'.  
 
-  Definition state := disk value.
+  Definition state' := disk value.
   
-  Inductive prog : Type -> Type :=
-  | Read : addr -> prog (option value)
-  | Write : addr -> value -> prog unit.
+  Inductive prog' : Type -> Type :=
+  | Read : addr -> prog' (option value)
+  | Write : addr -> value -> prog' unit.
 
   
-  Inductive exec :
-    forall T, oracle ->  state -> prog T -> @Result state T -> Prop :=
+  Inductive exec' :
+    forall T, oracle' ->  state' -> prog' T -> @Result state' T -> Prop :=
   | ExecRead : 
       forall d a,
-        exec [Cont] d (Read a) (Finished d (d a))
+        exec' [Cont] d (Read a) (Finished d (d a))
              
   | ExecWrite :
       forall d a v,
-        exec [Cont] d (Write a v) (Finished (upd d a v) tt)
+        exec' [Cont] d (Write a v) (Finished (upd d a v) tt)
 
   | ExecCrash :
-      forall T d (p: prog T),
-        exec [Crash] d p (Crashed d).
+      forall T d (p: prog' T),
+        exec' [Crash] d p (Crashed d).
 
-  Hint Constructors exec : core.
+  Hint Constructors exec' : core.
   
-  Definition weakest_precondition T (p: prog T) :=
-   match p in prog T' return (T' -> state -> Prop) -> oracle -> state -> Prop with
+  Definition weakest_precondition' T (p: prog' T) :=
+   match p in prog' T' return (T' -> state' -> Prop) -> oracle' -> state' -> Prop with
    | Read a =>
      (fun Q o s =>
         o = [Cont] /\
@@ -48,13 +48,13 @@ Set Implicit Arguments.
         Q tt (upd s a v))
    end.
 
-  Definition weakest_crash_precondition T (p: prog T) :=
-   fun (Q: state -> Prop) o (s: state) => o = [Crash] /\ Q s.
+  Definition weakest_crash_precondition' T (p: prog' T) :=
+   fun (Q: state' -> Prop) o (s: state') => o = [Crash] /\ Q s.
 
-  Theorem wp_complete:
-    forall T (p: prog T) H Q,
-      (forall o s, H o s -> weakest_precondition p Q o s) <->
-      (forall o s, H o s -> (exists s' v, exec o s p (Finished s' v) /\ Q v s')).
+  Theorem wp_complete':
+    forall T (p: prog' T) H Q,
+      (forall o s, H o s -> weakest_precondition' p Q o s) <->
+      (forall o s, H o s -> (exists s' v, exec' o s p (Finished s' v) /\ Q v s')).
   Proof.
     intros; destruct p; simpl; eauto;
     split; intros;
@@ -64,12 +64,12 @@ Set Implicit Arguments.
     inversion H0; cleanup; eauto.
   Qed.
   
-  Theorem wcp_complete:
-    forall T (p: prog T) H C,
-      (forall o s, H o s -> weakest_crash_precondition p C o s) <->
-      (forall o s, H o s -> (exists s', exec o s p (Crashed s') /\ C s')).
+  Theorem wcp_complete':
+    forall T (p: prog' T) H C,
+      (forall o s, H o s -> weakest_crash_precondition' p C o s) <->
+      (forall o s, H o s -> (exists s', exec' o s p (Crashed s') /\ C s')).
   Proof.
-    unfold weakest_crash_precondition;
+    unfold weakest_crash_precondition';
     intros; destruct p; simpl; eauto;
     split; intros;
     specialize H0 with (1:= X);
@@ -78,30 +78,30 @@ Set Implicit Arguments.
     inversion H0; cleanup; eauto.
   Qed.
 
-  Theorem exec_deterministic_wrt_oracle :
-    forall o s T (p: prog T) ret1 ret2,
-      exec o s p ret1 ->
-      exec o s p ret2 ->
+  Theorem exec_deterministic_wrt_oracle' :
+    forall o s T (p: prog' T) ret1 ret2,
+      exec' o s p ret1 ->
+      exec' o s p ret2 ->
       ret1 = ret2.
   Proof.
     intros; destruct p; simpl in *; cleanup;
     repeat
       match goal with
-      | [H: exec _ _ _ _ |- _] =>
+      | [H: exec' _ _ _ _ |- _] =>
         inversion H; clear H; cleanup
       end; eauto.
   Qed.
   
   Definition CacheOperation :=
     Build_Operation
-      (list_eq_dec token_dec)
-      prog
-      exec
-      weakest_precondition
-      weakest_crash_precondition
-      wp_complete
-      wcp_complete
-      exec_deterministic_wrt_oracle.
+      (list_eq_dec token_dec')
+      prog'
+      exec'
+      weakest_precondition'
+      weakest_crash_precondition'
+      wp_complete'
+      wcp_complete'
+      exec_deterministic_wrt_oracle'.
 
   Definition CacheLang := Build_Language CacheOperation.
   Definition CacheHL := Build_HoareLogic CacheLang.
