src/Layers/LoggedDiskLayer/Definitions.v
@@ -3,50 +3,50 @@ Import ListNotations.
 
 Set Implicit Arguments.
   
-  Inductive token :=
-  | CrashBefore : token
-  | CrashAfter : token
-  | Cont : token.
+  Inductive token' :=
+  | CrashBefore : token'
+  | CrashAfter : token'
+  | Cont : token'.
 
-  Definition token_dec : forall (t t': token), {t=t'}+{t<>t'}.
+  Definition token_dec' : forall (t t': token'), {t=t'}+{t<>t'}.
     decide equality.
   Defined.
 
-  Definition oracle := list token.  
+  Definition oracle' := list token'.  
 
-  Definition state := disk (set value).
+  Definition state' := disk (set value).
   
-  Inductive prog : Type -> Type :=
-  | Read : addr -> prog value
-  | Write : list addr -> list value -> prog unit.
+  Inductive prog' : Type -> Type :=
+  | Read : addr -> prog' value
+  | Write : list addr -> list value -> prog' unit.
    
-  Inductive exec :
-    forall T, oracle ->  state -> prog T -> @Result state T -> Prop :=
+  Inductive exec' :
+    forall T, oracle' ->  state' -> prog' T -> @Result state' T -> Prop :=
   | ExecRead : 
       forall d a v,
         read d a = Some v ->
-        exec [Cont] d (Read a) (Finished d v)
+        exec' [Cont] d (Read a) (Finished d v)
              
   | ExecWrite :
       forall d la lv,
-        exec [Cont] d (Write la lv) (Finished (write_all d la lv) tt)
+        exec' [Cont] d (Write la lv) (Finished (write_all d la lv) tt)
 
   | ExecCrashRead :
       forall d a,
-        exec [CrashBefore] d (Read a) (Crashed d)
+        exec' [CrashBefore] d (Read a) (Crashed d)
   
   | ExecCrashWriteBefore :
       forall d la lv,
-        exec [CrashBefore] d (Write la lv) (Crashed d)
+        exec' [CrashBefore] d (Write la lv) (Crashed d)
 
   | ExecCrashWriteAfter :
       forall d la lv,
-        exec [CrashAfter] d (Write la lv) (Crashed (write_all d la lv)).
+        exec' [CrashAfter] d (Write la lv) (Crashed (write_all d la lv)).
 
-  Hint Constructors exec : core.
+  Hint Constructors exec' : core.
 
-   Definition weakest_precondition T (p: prog T) :=
-   match p in prog T' return (T' -> state -> Prop) -> oracle -> state -> Prop with
+   Definition weakest_precondition' T (p: prog' T) :=
+   match p in prog' T' return (T' -> state' -> Prop) -> oracle' -> state' -> Prop with
    | Read a =>
      (fun Q o s =>
        exists v,
@@ -59,8 +59,8 @@ Set Implicit Arguments.
        Q tt (write_all s la lv))
    end.
 
-  Definition weakest_crash_precondition T (p: prog T) :=
-    match p in prog T' return (state -> Prop) -> oracle -> state -> Prop with
+  Definition weakest_crash_precondition' T (p: prog' T) :=
+    match p in prog' T' return (state' -> Prop) -> oracle' -> state' -> Prop with
    | Read a =>
      (fun Q o s =>
          o = [CrashBefore] /\
@@ -73,10 +73,10 @@ Set Implicit Arguments.
         Q (write_all s la lv)))
    end.
 
-  Theorem wp_complete:
-    forall T (p: prog T) H Q,
-      (forall o s, H o s -> weakest_precondition p Q o s) <->
-      (forall o s, H o s -> (exists s' v, exec o s p (Finished s' v) /\ Q v s')).
+  Theorem wp_complete':
+    forall T (p: prog' T) H Q,
+      (forall o s, H o s -> weakest_precondition' p Q o s) <->
+      (forall o s, H o s -> (exists s' v, exec' o s p (Finished s' v) /\ Q v s')).
   Proof.
     intros; destruct p; simpl; eauto;
     split; intros;
@@ -86,12 +86,12 @@ Set Implicit Arguments.
     inversion H0; cleanup; eauto.
   Qed.
   
-  Theorem wcp_complete:
-    forall T (p: prog T) H C,
-      (forall o s, H o s -> weakest_crash_precondition p C o s) <->
-      (forall o s, H o s -> (exists s', exec o s p (Crashed s') /\ C s')).
+  Theorem wcp_complete':
+    forall T (p: prog' T) H C,
+      (forall o s, H o s -> weakest_crash_precondition' p C o s) <->
+      (forall o s, H o s -> (exists s', exec' o s p (Crashed s') /\ C s')).
   Proof.
-    unfold weakest_crash_precondition;
+    unfold weakest_crash_precondition';
     intros; destruct p; simpl; eauto;
     split; intros;
     specialize H0 with (1:= X);
@@ -99,52 +99,31 @@ Set Implicit Arguments.
 
     inversion H0; cleanup; eauto.
   Qed.
-  
-  Fixpoint oracle_ok T (p: prog T) o (s: state) :=
-    match p with
-    |Read _ =>
-     o = [Cont] \/ o = [CrashBefore]
-    |Write _ _ =>
-     o = [Cont] \/ o = [CrashBefore] \/ o = [CrashAfter]
-    end.
 
-  Theorem exec_deterministic_wrt_oracle :
-    forall o s T (p: prog T) ret1 ret2,
-      exec o s p ret1 ->
-      exec o s p ret2 ->
+  Theorem exec_deterministic_wrt_oracle' :
+    forall o s T (p: prog' T) ret1 ret2,
+      exec' o s p ret1 ->
+      exec' o s p ret2 ->
       ret1 = ret2.
   Proof.
     intros; destruct p; simpl in *; cleanup;
     repeat
       match goal with
-      | [H: exec _ _ _ _ |- _] =>
-        inversion H; clear H; cleanup
-      end; eauto.
-  Qed.
-
-  Theorem exec_then_oracle_ok:
-    forall T (p: prog T) o s r,
-      exec o s p r ->
-      oracle_ok p o s.
-  Proof.
-    intros; destruct p; simpl in *; cleanup;
-    repeat
-      match goal with
-      | [H: exec _ _ _ _ |- _] =>
+      | [H: exec' _ _ _ _ |- _] =>
         inversion H; clear H; cleanup
       end; eauto.
   Qed.
   
   Definition LoggedDiskOperation :=
     Build_Operation
-      (list_eq_dec token_dec)
-      prog
-      exec
-      weakest_precondition
-      weakest_crash_precondition
-      wp_complete
-      wcp_complete
-      exec_deterministic_wrt_oracle.
+      (list_eq_dec token_dec')
+      prog'
+      exec'
+      weakest_precondition'
+      weakest_crash_precondition'
+      wp_complete'
+      wcp_complete'
+      exec_deterministic_wrt_oracle'.
 
   Definition LoggedDiskLang := Build_Language LoggedDiskOperation.
   Definition LoggedDiskHL := Build_HoareLogic LoggedDiskLang.
